\chapter{Equations}

\begin{enumerate}
\item equation+aligned
\begin{equation}
\begin{aligned}
& \text{minimize}
& & C=\sum_{i,j=1}^{n}c_{ij}x_{ij} \\
& \text{subject to}
& & \sum_{i,j=1}^{n}x_{ji}+b_{i}=\sum_{i,j=1}^{n}x_{ij},\; 1^{T}b=0 \\
&&& l_{ij}\leq x_{ij}\leq u_{ij}.
\end{aligned}
\end{equation}
\begin{lstlisting}[language=Tex]
\begin{equation}
\begin{aligned}
& \text{minimize}
& & C=\sum_{i,j=1}^{n}c_{ij}x_{ij} \\
& \text{subject to}
& & \sum_{i,j=1}^{n}x_{ji}+b_{i}=\sum_{i,j=1}^{n}x_{ij},\; 1^{T}b=0 \\
&&& l_{ij}\leq x_{ij}\leq u_{ij}.
\end{aligned}
\end{equation}
\end{lstlisting}

\item align
\begin{align}
& \text{minimize}
& & c^{T}x+b \\
& \text{subject to}
& & Gx\preceq h \\
&&& Ax=b,
\end{align}

\begin{lstlisting}[language=Tex]
\begin{align}
& \text{minimize}
& & c^{T}x+b \\
& \text{subject to}
& & Gx\preceq h \\
&&& Ax=b,
\end{align}
\end{lstlisting}

\item align+aligned
\begin{align}
\begin{aligned}
& \text{minimize}
& & c^{T}x+b \\
& \text{subject to}
& & Gx\preceq h \\
&&& Ax=b,
\end{aligned}
\end{align}

\begin{lstlisting}[language=Tex]
\begin{align}
\begin{aligned}
& \text{minimize}
& & c^{T}x+b \\
& \text{subject to}
& & Gx\preceq h \\
&&& Ax=b,
\end{aligned}
\end{align}
\end{lstlisting}

\item align
\begin{align}
\max\limits_{n_1,n_2,...,n_k}
&\text{\quad}\sum_{i=1}^{K}(1-\text{exp}(-\lambda n_i R_i)),\label{eq1}\\
\text{subject to}
&\text{\quad}\sum_{i=1}^{K}n_ix-LB \leq 0,\label{eq2}\\
&\text{\quad} n_i-L \leq 0,\forall i,\label{eq3}\\
&\text{\quad} n_i \geq 1, \forall i.\label{eq4}
\end{align}

\begin{lstlisting}[language=Tex]
\begin{align}
\max\limits_{n_1,n_2,...,n_k}
&\text{\quad}\sum_{i=1}^{K}(1-\text{exp}(-\lambda n_i R_i)),\label{eq1}\\
\text{subject to}
&\text{\quad}\sum_{i=1}^{K}n_ix-LB \leq 0,\label{eq2}\\
&\text{\quad} n_i-L \leq 0,\forall i,\label{eq3}\\
&\text{\quad} n_i \geq 1, \forall i.\label{eq4}
\end{align}
\end{lstlisting}

\item align$^{\ast}$
\begin{align*}
L(x,\lambda ,\nu )& =c^{T}x+\lambda ^{T}(Gx-h)+\nu ^{T}(Ax-b) \\
& =(c^{T}+\lambda^{T}G+\nu ^{T}A)x-\lambda ^{T}h-\nu ^{T}b.
\end{align*}

\begin{lstlisting}[language=Tex]
\begin{align*}
L(x,\lambda ,\nu )& =c^{T}x+\lambda ^{T}(Gx-h)+\nu ^{T}(Ax-b) \\
& =(c^{T}+\lambda^{T}G+\nu ^{T}A)x-\lambda ^{T}h-\nu ^{T}b.
\end{align*}
\end{lstlisting}

\item align
\begin{align}
& \max \sum\limits_i^{} {Q_i^s (t)\mu (i,t)}  \\
& \max \sum\limits_i^{} {Q_i^s (t)\min \{ Q_i^s (t),\mu (i,t)} \}  \\
& \max \sum\limits_i^{} {(Q_i^s (t))^2  - } (Q_i^e (t))^2
\end{align}

\begin{lstlisting}[language=Tex]
\begin{align}
& \max \sum\limits_i^{} {Q_i^s (t)\mu (i,t)}  \\
& \max \sum\limits_i^{} {Q_i^s (t)\min \{ Q_i^s (t),\mu (i,t)} \}  \\
& \max \sum\limits_i^{} {(Q_i^s (t))^2  - } (Q_i^e (t))^2
\end{align}
\end{lstlisting}

\item equation
\begin{equation}
g(\lambda ,\nu )=\inf_{x}L(x,\lambda ,\nu )=-\lambda ^{T}h-\nu
^{T}b+\inf_{x}(c^{T}+\lambda ^{T}G+\nu ^{T}A)x
\end{equation}

\begin{lstlisting}[language=Tex]
\begin{equation}
g(\lambda ,\nu )=\inf_{x}L(x,\lambda ,\nu )=-\lambda ^{T}h-\nu
^{T}b+\inf_{x}(c^{T}+\lambda ^{T}G+\nu ^{T}A)x
\end{equation}
\end{lstlisting}

\item equation$^{\ast}$
\begin{equation*}
\Delta w_{s}(t)=\frac{x_{s}(t)(1-q_{s}(t))}{w_{s}}-\frac{%
w_{s}(t)x_{s}(t)q_{s}(t)}{2}\times \frac{4}{3}
\end{equation*}

\begin{lstlisting}[language=Tex]
\begin{equation*}
\Delta w_{s}(t)=\frac{x_{s}(t)(1-q_{s}(t))}{w_{s}}-\frac{%
w_{s}(t)x_{s}(t)q_{s}(t)}{2}\times \frac{4}{3}
\end{equation*}
\end{lstlisting}

\item equation$^{\ast}$+cases
\begin{equation*}
g(\lambda ,\nu )=
\begin{cases} -\lambda ^{T}h-\nu ^{T}b & c^{T}+\lambda ^{T}G+\nu ^{T}A=0
\\
-\infty &\text{otherwise.}
\end{cases}
\end{equation*}

\begin{lstlisting}[language=Tex]
\begin{equation*}
g(\lambda ,\nu )=
\begin{cases} -\lambda ^{T}h-\nu ^{T}b & c^{T}+\lambda ^{T}G+\nu ^{T}A=0
\\
-\infty &\text{otherwise.}
\end{cases}
\end{equation*}
\end{lstlisting}

\item align$^{\ast}$+intertext
\begin{align*}
U_{s}(x_{s})& =\int f_{s}(x_{s})dx_{s} \\
\intertext{text you want}\\
& =\int q_{s}dx_{s}\\
& =\int \frac{3}{2x_{s}^{2}D_{s}^{2}+3}dx_{s}\\
& =\frac{\sqrt{\frac{3}{2}}}{D_{s}}\tan ^{-1}(%
\sqrt{\frac{2}{3}}x_{s}D_{s})
\end{align*}

\begin{lstlisting}[language=Tex]
\begin{align*}
U_{s}(x_{s})& =\int f_{s}(x_{s})dx_{s} \\
\intertext{text you want}\\
& =\int q_{s}dx_{s}\\
& =\int \frac{3}{2x_{s}^{2}D_{s}^{2}+3}dx_{s}\\
& =\frac{\sqrt{\frac{3}{2}}}{D_{s}}\tan ^{-1}(%
\sqrt{\frac{2}{3}}x_{s}D_{s})
\end{align*}
\end{lstlisting}

\item align with intertext
\begin{align}
\intertext{For $m=1$,}\\
(A^{1})^{-1}& =(A)^{-1}=(A^{-1})^{1}\\
\intertext{Assume the result holds in the case $m=k$, that is,}\\
(A^{k})^{-1}& =(A^{-1})^{k}\\
\intertext{It follows that}\\
(A^{-1})^{k+1}A^{k+1}& =A^{-1}(A^{-1})^{k}A^{k}A=A^{-1}A=I\\
\intertext{and}\\
A^{k+1}(A^{-1})^{k+1}& =AA^{k}(A^{-1})^{k}A^{-1}=AA^{-1}=I\\
\intertext{Therefore}\\
(A^{-1})^{k+1}& =(A^{k+1})^{-1}
\end{align}

\begin{lstlisting}[language=Tex]
\begin{align}
\intertext{For $m=1$,}\\
(A^{1})^{-1}& =(A)^{-1}=(A^{-1})^{1}\\
\intertext{Assume the result holds in the case $m=k$, that is,}\\
(A^{k})^{-1}& =(A^{-1})^{k}\\
\intertext{It follows that}\\
(A^{-1})^{k+1}A^{k+1}& =A^{-1}(A^{-1})^{k}A^{k}A=A^{-1}A=I\\
\intertext{and}\\
A^{k+1}(A^{-1})^{k+1}& =AA^{k}(A^{-1})^{k}A^{-1}=AA^{-1}=I\\
\intertext{Therefore}\\
(A^{-1})^{k+1}& =(A^{k+1})^{-1}
\end{align}
\end{lstlisting}

\item max with under var
\begin{equation*}
\begin{aligned}
& \max\limits_{n_1,n_2,...,n_k}
& & \sum_{i=1}^{K}(1-\text{exp}(-\lambda n_i R_i)),\\
& \text{subject to}
& & \sum_{i=1}^{K}n_ix-LB \leq 0, \\
&&& n_i-L \leq 0,\forall i,\\
&&& n_i \geq 1, \forall i.
\end{aligned}
\end{equation*}

\begin{lstlisting}[language=Tex]
\begin{equation*}
\begin{aligned}
& \max\limits_{n_1,n_2,...,n_k}
& & \sum_{i=1}^{K}(1-\text{exp}(-\lambda n_i R_i)),\\
& \text{subject to}
& & \sum_{i=1}^{K}n_ix-LB \leq 0, \\
&&& n_i-L \leq 0,\forall i,\\
&&& n_i \geq 1, \forall i.
\end{aligned}
\end{equation*}
\end{lstlisting}

\item BB fonts
$\mathbb{N,R,Z}$

\begin{lstlisting}[language=Tex]
$\mathbb{N,R,Z}$
\end{lstlisting}

\item cal fonts
$\mathcal{IDP}$
\begin{lstlisting}[language=Tex]
$\mathcal{IDP}$
\end{lstlisting}
\end{enumerate}